More work on dns packet encoder example

src/BinEncoders/Examples/Dns.v
@@ -3,29 +3,24 @@ Require Import Coq.Strings.String
 Require Import Fiat.BinEncoders.Specs
                Fiat.BinEncoders.Libraries.Core
                Fiat.BinEncoders.Libraries.FixInt
-               Fiat.BinEncoders.Libraries.Char.
+               Fiat.BinEncoders.Libraries.Char
+               Fiat.BinEncoders.Libraries.VList.
 
 Set Implicit Arguments.
 
 Section DnsPacket.
 
-  Variable List_encode : forall (A : Type) (encode_A : A -> bin), list A -> bin.
-
   Inductive RRecordType := A | CNAME | NS | MX.
   Inductive RRecordClass := IN | CH | HS.
 
-  Record question :=
-    { qname : list (list ascii);
-      qtype : RRecordType;
-      qclass : RRecordClass }.
-
+  (* find a way to do this systematically *)
   Definition RRecordTypeToFixInt (t : RRecordType) : {n | (n < exp2 16)%N}.
     refine (match t with
             | A     => exist _ (1%N) _
             | CNAME => exist _ (5%N) _
             | NS    => exist _ (2%N) _
             | MX    => exist _ (15%N) _
-            end); admit.
+            end); rewrite <- N.compare_lt_iff; eauto.
   Defined.
 
   Definition RRecordClassToFixInt (c : RRecordClass) : {n | (n < exp2 16)%N}.
@@ -33,23 +28,35 @@ Section DnsPacket.
             | IN => exist _ (1%N) _
             | CH => exist _ (3%N) _
             | HS => exist _ (4%N) _
-            end); admit.
+            end); rewrite <- N.compare_lt_iff; eauto.
   Defined.
 
-  Global Instance T_decoder
-    : decoder (fun _ => True) RRecordTypeToFixInt.
-  Admitted.
+  Global Instance RRType_decoder
+    : decoder (fun _ => True) RRecordTypeToFixInt :=
+    { decode := fun n => if N.eq_dec (proj1_sig n) (1%N) then A
+                         else if N.eq_dec (proj1_sig n) (5%N) then CNAME
+                         else if N.eq_dec (proj1_sig n) (2%N) then NS
+                         else MX;
+      decode_correct := _ }.
+  Proof.
+    intros data _; destruct data; eauto.
+  Defined.
 
-  Global Instance C_decoder
-    : decoder (fun _ => True) RRecordClassToFixInt.
-  Admitted.
+  Global Instance RRClass_decoder
+    : decoder (fun _ => True) RRecordClassToFixInt :=
+    { decode := fun n => if N.eq_dec (proj1_sig n) (1%N) then IN
+                         else if N.eq_dec (proj1_sig n) (3%N) then CH
+                         else HS;
+      decode_correct := _ }.
+  Proof.
+    intros data _; destruct data; eauto.
+  Defined.
 
-  Global Instance List_decoder
-         (A : Type)
-         (encode_A : A -> bin)
-         (A_Decoder : decoder (fun _ => True) encode_A)
-    : decoder (fun _ => True) (List_encode encode_A).
-  Admitted.
+
+  Record question :=
+    { qname : list (list ascii);
+      qtype : RRecordType;
+      qclass : RRecordClass }.
 
   Global Instance App_decoder
          (A : Type)
@@ -59,24 +66,8 @@ Section DnsPacket.
               (fun _bundle : A * bin => let (_data, _bin) := _bundle in encode_A _data ++ _bin).
   Admitted.
 
-  Global Instance App_decoder'
-         (A : Type)
-         (encode_A : A -> bin)
-         (A_Decoder : decoder (fun _ => True) encode_A)
-    : decoder (fun _ => True)
-              (fun _bundle : A * bin => let (_data, _) := _bundle in encode_A _data).
-  Admitted.
-
-  Global Instance NestedDecoder A B C
-         (encodeA : A -> B)
-         (encodeB : B -> C)
-         (A_decoder : decoder (fun _ => True) encodeA)
-         (B_decoder : decoder (fun _ => True) encodeB)
-    : decoder (fun _ => True) (fun data => encodeB (encodeA data)).
-  Admitted.
-
   Definition question_encode (q : question) :=
-    List_encode (List_encode Char_encode) (qname q) ++
+    VList_encode (VList_encode_pair Char_encode_pair) (qname q) ++
     FixInt_encode _ (RRecordTypeToFixInt (qtype q)) ++
     FixInt_encode _ (RRecordClassToFixInt (qclass q)).
 
@@ -92,42 +83,48 @@ Section DnsPacket.
            (encode1:=fun (_bundle : _ * bin) =>
                        let (_proj, _bin) := _bundle
                        in  e1 _proj ++ _bin)
-           (encode2:=e2)
     end.
     instantiate (1:=fun _ => True). intuition. cbv beta. eapply decode_correct. intro.
 
     match goal with
-    | |- encode_decode_correct _ (fun data => ?e1 (?p1 (qtype data)) ++ @?e2 data) _ =>
+    | |- encode_decode_correct _ (fun data => ?e1 (?p1 (_ data)) ++ @?e2 data) _ =>
         eapply decode_unpack with
            (encode1:=fun (_bundle : _ * bin) =>
                        let (_proj, _bin) := _bundle
                        in  e1 (p1 _proj) ++ _bin)
-           (encode2:=e2)
     end.
     instantiate (1:=fun _ => True). intuition. cbv beta. eapply decode_correct. intro.
 
+    (* final step! *)
+    eapply decode_moveproj with
+      (encode:=fun c => FixInt_encode 16 (RRecordClassToFixInt c))
+      (constr:=fun _ => Build_question _ _ _).
+    instantiate (1:=fun _ => True). intuition. cbv beta. eapply decode_correct. intro.
+    intros. destruct data.
+    intuition. simpl in *. subst. reflexivity.
+
+    (*
     match goal with
-    | |- encode_decode_correct _ (fun data => ?e1 (?p1 (qclass data))) _ =>
+    | |- encode_decode_correct _ (fun data => ?e1 (?p1 (_ data)) ++ @?e2 data) _ =>
         eapply decode_unpack with
            (encode1:=fun (_bundle : _ * bin) =>
-                       let (_proj, _) := _bundle
-                       in  e1 (p1 _proj))
-           (encode2:=fun _ => nil)
+                       let (_proj, _bin) := _bundle
+                       in  e1 (p1 _proj) ++ _bin)
     end.
     instantiate (1:=fun _ => True). intuition. cbv beta. eapply decode_correct. intro.
-
     unfold encode_decode_correct.
     intros. destruct data.
     instantiate (1:=fun _ _ => Build_question _ _ _). simpl.
-    simpl in *. intuition. subst. reflexivity.
+    simpl in *. intuition. subst. reflexivity. *)
+
   Defined.
 
   Record packet :=
     { id : Bvector 16;
       flags : Bvector 16;
-      questions : nat;
-      answers : nat;
-      authority : list nat;
-      additional : list nat }.
+      questions : list question;
+      answers : list question;
+      authority : list question;
+      additional : list question }.
 
 End DnsPacket.
