src/BinEncoders/Libraries/Char.v
@@ -8,28 +8,41 @@ Section Char_encode_decode.
 
   Lemma nonzero_8 : 0 < 8. omega. Qed.
 
-  Definition Char_encode (c : ascii) : bin.
-    refine (FixInt_encode 8 (exist _ (N_of_ascii c) _)).
+  Definition Char_encode_pair (p : ascii * bin) : bin.
+    refine (FixInt_encode_pair 8 (exist _ (N_of_ascii (fst p)) _, snd p)).
     unfold exp2; unfold exp2'.
-    induction c.
+    induction (fst p).
     repeat (match goal with
               | B : bool |- _ => destruct B
             end); simpl; unfold Nlt; auto.
   Defined.
 
-  Definition Char_decode (b : bin) : ascii :=
-    ascii_of_N (proj1_sig (@Specs.decode _ _ _ _ (FixInt_decoder 8) b)).
+  Definition Char_encode (c : ascii) := Char_encode_pair (c, nil).
+
+  Definition Char_decode_pair (b : bin) : ascii * bin :=
+    let (_n, _bin) := @Specs.decode _ _ _ _ (FixInt_decoder_pair 8) b
+    in  (ascii_of_N (proj1_sig _n), _bin).
+
+  Definition Char_decode (b : bin) : ascii := fst (Char_decode_pair b).
+
+  Theorem Char_encode_decode_correct_pair :
+    encode_decode_correct (fun _ => True) Char_encode_pair Char_decode_pair.
+  Proof.
+    unfold encode_decode_correct, Char_encode_pair, Char_decode_pair.
+    intros c _.
+    rewrite (@decode_correct _ _ _ (FixInt_encode_pair 8) _); simpl; eauto.
+    rewrite ascii_N_embedding; intuition.
+  Qed.
 
   Theorem Char_encode_decode_correct :
     encode_decode_correct (fun _ => True) Char_encode Char_decode.
   Proof.
     unfold encode_decode_correct, Char_encode, Char_decode.
     intros c _.
-    rewrite (@decode_correct _ _ _ (FixInt_encode 8) _); simpl; eauto.
-    rewrite ascii_N_embedding; eauto.
+    rewrite Char_encode_decode_correct_pair; intuition.
   Qed.
 
-  (*Theorem decode_shorten : decode_shorten decode.
+  (* Theorem decode_shorten : decode_shorten decode.
   Proof.
     unfold decode_shorten, decode; intro ls.
     pose proof (shorten_R (FixInt_encode_decode 8 nonzero_8) ls).
@@ -48,3 +61,8 @@ Global Instance Char_decoder
   : decoder (fun _ => True) Char_encode :=
   { decode := Char_decode;
     decode_correct := Char_encode_decode_correct }.
+
+Global Instance Char_decoder_pair
+  : decoder (fun _ => True) Char_encode_pair :=
+  { decode := Char_decode_pair;
+    decode_correct := Char_encode_decode_correct_pair }.
