src/BinEncoders/Libraries/List.v
@@ -16,16 +16,29 @@ Section List_encode_decode.
     | x :: xs => encode_A (x, List_encode xs)
     end.
 
-  Fixpoint List_decode (size : nat) (b : bin) :=
+  Definition List_encode_pair (p : list A * bin) :=
+    List_encode (fst p) ++ snd p.
+
+  Fixpoint List_decode_pair (size : nat) (b : bin) :=
     match size with
-    | O => nil
-    | S size' => let (_data, _bin) := @decode _ _ _ _ A_Decoder b
-                 in  _data :: List_decode size' _bin
+    | O => (nil, b)
+    | S size' => let (_data, _bin) := @decode _ _ _ _ A_Decoder b in
+                 let (_rest, __bin) := List_decode_pair size' _bin in
+                     (_data :: _rest, __bin)
     end.
+
+  Definition List_decode (size : nat) (b : bin) :=
+    fst (List_decode_pair size b).
 
   Lemma List_encode_decode_correct :
     forall size, encode_decode_correct
                    (fun data : list A => length data = size) List_encode (List_decode size).
+  Proof.
+  Admitted.
+
+  Lemma List_encode_decode_correct_pair :
+    forall size, encode_decode_correct
+                   (fun data => length (fst data) = size) List_encode_pair (List_decode_pair size).
   Proof.
   Admitted.
 
@@ -39,3 +52,12 @@ Global Instance List_decoder
   : decoder (fun data => length data = size) (List_encode encode_A) :=
   { decode := List_decode A_Decoder size;
     decode_correct := @List_encode_decode_correct _ encode_A A_Decoder size }.
+
+Global Instance List_decoder_pair
+       (A : Type)
+       (encode_A : A * bin -> bin)
+       (A_Decoder : decoder (fun _ => True) encode_A)
+       (size : nat)
+  : decoder (fun data => length (fst data) = size) (List_encode_pair encode_A) :=
+  { decode := List_decode_pair A_Decoder size;
+    decode_correct := @List_encode_decode_correct_pair _ encode_A A_Decoder size }.
