src/BinEncoders/Libraries/VList.v
@@ -1,0 +1,53 @@
+Require Export Coq.Lists.List.
+Require Import Fiat.BinEncoders.Specs
+               Fiat.BinEncoders.Libraries.Core.
+
+Set Implicit Arguments.
+
+Section VList_encode_decode.
+
+  Variable (A : Type)
+           (encode_A : A * bin -> bin)
+           (A_Decoder : decoder (fun _ => True) encode_A).
+
+  Fixpoint VList_encode (ls : list A) :=
+    match ls with
+    | nil => nil
+    | x :: xs => encode_A (x, VList_encode xs)
+    end.
+
+  Definition VList_encode_pair (p : list A * bin) :=
+    VList_encode (fst p) ++ snd p.
+
+  Fixpoint VList_decode_pair (b : bin) : list A * bin := (nil, b).
+
+  Definition VList_decode (b : bin) :=
+    fst (VList_decode_pair b).
+
+  Lemma VList_encode_decode_correct :
+    encode_decode_correct (fun _ => True) VList_encode VList_decode.
+  Proof.
+  Admitted.
+
+  Lemma List_encode_decode_correct_pair :
+    encode_decode_correct (fun _ => True) VList_encode_pair VList_decode_pair.
+  Proof.
+  Admitted.
+
+End VList_encode_decode.
+
+Global Instance VList_decoder
+       (A : Type)
+       (encode_A : A * bin -> bin)
+       (A_Decoder : decoder (fun _ => True) encode_A)
+  : decoder (fun _ => True) (VList_encode encode_A) :=
+  { decode := VList_decode _;
+    decode_correct := @VList_encode_decode_correct _ encode_A }.
+
+Global Instance VList_decoder_pair
+       (A : Type)
+       (encode_A : A * bin -> bin)
+       (A_Decoder : decoder (fun _ => True) encode_A)
+  : decoder (fun _ => True) (VList_encode_pair encode_A) :=
+  { decode := VList_decode_pair _;
+    decode_correct := @List_encode_decode_correct_pair _ encode_A }.
